CBS.h
@@ -21,6 +21,8 @@ bool CBS_cbs_get_u(CBS_cbs_t *cbs, uint32_t *out, uint32_t num);
 
 bool CBS_cbs_get_u8(CBS_cbs_t *cbs, uint8_t *out);
 
+bool CBS_cbs_get_u16(CBS_cbs_t *cbs, uint16_t *out);
+
 bool CBS_cbs_get_u24(CBS_cbs_t *cbs, uint32_t *out);
 
 bool CBS_cbs_get_u32(CBS_cbs_t *cbs, uint32_t *out);
