CBS.fst
@@ -30,11 +30,11 @@ let rec big_endian (b:seq U8.t) : Tot (n:nat) (decreases (Seq.length b)) =
 
 val cbs_get_u :
   cbs: buffer cbs_t{length cbs = 1} ->
-  out: buffer U32.t{length out = 1} ->
+  out: buffer U32.t{length out = 1 /\ disjoint cbs out} -> // TODO disjoint
   num: U32.t{U32.(v num > 0 /\ v num < 5)} ->
   ST bool
   (requires (fun h -> live h out /\ live h cbs /\ live h (get h cbs 0).data))
-  (ensures (fun h0 r h1 -> live h1 out /\ // modifies_1 out h0 h1 ?
+  (ensures (fun h0 r h1 -> live h0 out /\ live h1 out /\ modifies_1 out h0 h1 /\
     (let cbs0 = get h0 cbs 0 in
       // Return false if there aren't enough bytes.
       r == U32.(v cbs0.len >= v num) //\
@@ -44,8 +44,9 @@ val cbs_get_u :
 
 let cbs_get_u cbs out num =
   let cbs0 = cbs.(0ul) in
+  let h0 = FStar.HyperStack.ST.get() in
   if U32.(cbs0.len >=^ num) then (
-    let inv = (fun h _ -> live h out /\ live h cbs0.data) in
+    let inv = (fun h _ -> live h out /\ live h cbs0.data /\ modifies_1 out h0 h) in
     let f (i:U32.t{U32.(v 0ul <= v i /\ v i < v num)}) :
       Stack unit
         (requires (fun h -> live h out /\ live h cbs0.data))
@@ -69,7 +70,7 @@ val cbs_get_u8 :
       // Return false if there aren't enough bytes.
       r == (U32.v cbs0.len > 0) /\
       // If there are, the result will be cbs->data[0].
-      (not(r) \/ U8.v (get h1 out 0) == big_endian (slice (as_seq h0 cbs0.data) 0 1))
+      (~r \/ U8.v (get h1 out 0) == big_endian (slice (as_seq h0 cbs0.data) 0 1))
     )))
 
 let cbs_get_u8 cbs out =
@@ -81,13 +82,19 @@ let cbs_get_u8 cbs out =
     false
   )
 
-(*
 val cbs_get_u16 :
   cbs: buffer cbs_t{length cbs = 1} ->
-  out: buffer U16.t{length out = 1} ->
+  out: buffer U16.t{length out = 1 /\ disjoint cbs out} ->
   ST bool
-  (fun _ -> true)
-  (fun _ _ _ -> true)
+  (requires (fun h -> live h out /\ live h cbs /\ live h (get h cbs 0).data /\ Buffer.live h out))
+  (ensures (fun h0 r h1 -> live h0 out /\ live h1 out //\ modifies_1 out h0 h1
+    //(let cbs0 = get h0 cbs 0 in
+      // Return false if there aren't enough bytes.
+      //r == (U32.v cbs0.len > 1) //\
+      // If there are, check the result.
+      //(not(r) \/ U8.v (get h1 out 0) == big_endian (slice (as_seq h0 cbs0.data) 0 2))
+    //)
+    ))
 
 let cbs_get_u16 cbs out =
   push_frame ();
@@ -101,19 +108,18 @@ let cbs_get_u16 cbs out =
   ) in
   pop_frame();
   rv
-*)
 
 val cbs_get_u24 :
   cbs: buffer cbs_t{length cbs = 1} ->
-  out: buffer U32.t{length out = 1} ->
+  out: buffer U32.t{length out = 1 /\ disjoint cbs out} -> // TODO disjoint
   ST bool
   (requires (fun h -> live h out /\ live h cbs /\ live h (get h cbs 0).data))
-  (ensures (fun h0 r h1 -> live h1 out /\ // modifies_1 out h0 h1 /\
+  (ensures (fun h0 r h1 -> live h1 out /\ modifies_1 out h0 h1 /\
     (let cbs0 = get h0 cbs 0 in
       // Return false if there aren't enough bytes.
       r == (U32.v cbs0.len > 2) //\
       // If there are, check the result.
-      //(not(r) \/ U8.v (get h1 out 0) == big_endian (slice (as_seq h0 cbs0.data) 0 3))
+      //(not(r) \/ U32.v (get h1 out 0) == big_endian (slice (as_seq h0 cbs0.data) 0 3))
     )))
 
 let cbs_get_u24 cbs out =
@@ -121,15 +127,15 @@ let cbs_get_u24 cbs out =
 
 val cbs_get_u32 :
   cbs: buffer cbs_t{length cbs = 1} ->
-  out: buffer U32.t{length out = 1} ->
+  out: buffer U32.t{length out = 1 /\ disjoint cbs out} -> // TODO disjoint
   ST bool
   (requires (fun h -> live h out /\ live h cbs /\ live h (get h cbs 0).data))
-  (ensures (fun h0 r h1 -> live h1 out /\ // modifies_1 out h0 h1 /\
+  (ensures (fun h0 r h1 -> live h1 out /\ modifies_1 out h0 h1 /\
     (let cbs0 = get h0 cbs 0 in
       // Return false if there aren't enough bytes.
       r == (U32.v cbs0.len > 3) //\
       // If there are, check the result.
-      //(not(r) \/ U8.v (get h1 out 0) == big_endian (slice (as_seq h0 cbs0.data) 0 4))
+      //(not(r) \/ U32.v (get h1 out 0) == big_endian (slice (as_seq h0 cbs0.data) 0 4))
     )))
 
 let cbs_get_u32 cbs out =
